src/HOL/Subst/UTerm.thy
@@ -7,34 +7,31 @@ header{*Simple Term Structure for Unification*}
 
 theory UTerm
 imports Main
-
 begin
 
 text{*Binary trees with leaves that are constants or variables.*}
 
-datatype 'a uterm = Var 'a
-                  | Const 'a
-                  | Comb "'a uterm" "'a uterm"
+datatype 'a uterm =
+    Var 'a
+  | Const 'a
+  | Comb "'a uterm" "'a uterm"
 
-consts
-  vars_of  ::  "'a uterm => 'a set"
-  "<:"     ::  "'a uterm => 'a uterm => bool"   (infixl 54) 
-  uterm_size ::  "'a uterm => nat"
-
-syntax (xsymbols)
-  "op <:"     ::  "'a uterm => 'a uterm => bool"   (infixl "\<prec>" 54) 
-
-
+consts vars_of :: "'a uterm => 'a set"
 primrec
   vars_of_Var:   "vars_of (Var v) = {v}"
   vars_of_Const: "vars_of (Const c) = {}"
   vars_of_Comb:  "vars_of (Comb M N) = (vars_of(M) Un vars_of(N))"
 
+consts occs :: "'a uterm => 'a uterm => bool"   (infixl "<:" 54) 
+notation (xsymbols)
+  occs  (infixl "\<prec>" 54)
 primrec
   occs_Var:   "u \<prec> (Var v) = False"
   occs_Const: "u \<prec> (Const c) = False"
   occs_Comb:  "u \<prec> (Comb M N) = (u=M | u=N | u \<prec> M | u \<prec> N)"
 
+consts
+  uterm_size ::  "'a uterm => nat"
 primrec
   uterm_size_Var:   "uterm_size (Var v) = 0"
   uterm_size_Const: "uterm_size (Const c) = 0"
@@ -42,23 +39,22 @@ primrec
 
 
 lemma vars_var_iff: "(v \<in> vars_of(Var(w))) = (w=v)"
-by auto
+  by auto
 
 lemma vars_iff_occseq: "(x \<in> vars_of(t)) = (Var(x) \<prec> t | Var(x) = t)"
-by (induct_tac "t", auto)
+  by (induct t) auto
 
 
 text{* Not used, but perhaps useful in other proofs *}
-lemma occs_vars_subset [rule_format]: "M\<prec>N --> vars_of(M) \<subseteq> vars_of(N)"
-by (induct_tac "N", auto)
+lemma occs_vars_subset: "M\<prec>N \<Longrightarrow> vars_of(M) \<subseteq> vars_of(N)"
+  by (induct N) auto
 
 
 lemma monotone_vars_of:
-     "vars_of M Un vars_of N \<subseteq> (vars_of M Un A) Un (vars_of N Un B)"
-by blast
+    "vars_of M Un vars_of N \<subseteq> (vars_of M Un A) Un (vars_of N Un B)"
+  by blast
 
 lemma finite_vars_of: "finite(vars_of M)"
-by (induct_tac "M", auto)
-
+  by (induct M) auto
 
 end
