src/HOL/Subst/Subst.thy
@@ -11,92 +11,87 @@ imports AList UTerm
 begin
 
 consts
-
-  "=$="  ::  "[('a*('a uterm)) list,('a*('a uterm)) list] => bool" (infixr 52)
-  "<|"   ::  "'a uterm => ('a * 'a uterm) list => 'a uterm"        (infixl 55)
-  "<>"   ::  "[('a*('a uterm)) list, ('a*('a uterm)) list] 
-                 => ('a*('a uterm)) list"                          (infixl 56)
-  sdom   ::  "('a*('a uterm)) list => 'a set"
-  srange ::  "('a*('a uterm)) list => 'a set"
-
-
-syntax (xsymbols)
-  "op =$=" :: "[('a*('a uterm)) list,('a*('a uterm)) list] => bool" 
-              (infixr "\<doteq>" 52)
-  "op <|" :: "'a uterm => ('a * 'a uterm) list => 'a uterm" (infixl "\<lhd>" 55)
-  "op <>" :: "[('a*('a uterm)) list, ('a*('a uterm)) list] 
-                 => ('a*('a uterm)) list"                   (infixl "\<lozenge>" 56)
-
-
+  subst :: "'a uterm => ('a * 'a uterm) list => 'a uterm"  (infixl "<|" 55)
+notation (xsymbols)
+  subst  (infixl "\<lhd>" 55)
 primrec
   subst_Var:      "(Var v \<lhd> s) = assoc v (Var v) s"
   subst_Const:  "(Const c \<lhd> s) = Const c"
   subst_Comb:  "(Comb M N \<lhd> s) = Comb (M \<lhd> s) (N \<lhd> s)"
 
+definition
+  subst_eq :: "[('a*('a uterm)) list,('a*('a uterm)) list] => bool"  (infixr "=$=" 52) where
+  "r =$= s \<longleftrightarrow> (\<forall>t. t \<lhd> r = t \<lhd> s)"
+notation
+  subst_eq  (infixr "\<doteq>" 52)
 
-defs 
+definition
+  comp :: "[('a*('a uterm)) list, ('a*('a uterm)) list] => ('a*('a uterm)) list"
+    (infixl "<>" 56) where
+  "al <> bl = alist_rec al bl (%x y xs g. (x,y \<lhd> bl)#g)"
+notation
+  comp  (infixl "\<lozenge>" 56)
 
-  subst_eq_def:  "r =$= s == ALL t. t \<lhd> r = t \<lhd> s"
+definition
+  sdom :: "('a*('a uterm)) list => 'a set" where
+  "sdom al = alist_rec al {} (%x y xs g. if Var(x)=y then g - {x} else g Un {x})"
 
-  comp_def:    "al \<lozenge> bl == alist_rec al bl (%x y xs g. (x,y \<lhd> bl)#g)"
-
-  sdom_def:
-  "sdom(al) == alist_rec al {}  
-                (%x y xs g. if Var(x)=y then g - {x} else g Un {x})"
-
-  srange_def:
-   "srange(al) == Union({y. \<exists>x \<in> sdom(al). y = vars_of(Var(x) \<lhd> al)})"
+definition
+  srange :: "('a*('a uterm)) list => 'a set" where
+  "srange al = Union({y. \<exists>x \<in> sdom(al). y = vars_of(Var(x) \<lhd> al)})"
 
 
 
 subsection{*Basic Laws*}
 
 lemma subst_Nil [simp]: "t \<lhd> [] = t"
-by (induct_tac "t", auto)
+  by (induct t) auto
 
-lemma subst_mono [rule_format]: "t \<prec> u --> t \<lhd> s \<prec> u \<lhd> s"
-by (induct_tac "u", auto)
+lemma subst_mono: "t \<prec> u \<Longrightarrow> t \<lhd> s \<prec> u \<lhd> s"
+  by (induct u) auto
 
-lemma Var_not_occs [rule_format]:
-     "~ (Var(v) \<prec> t) --> t \<lhd> (v,t \<lhd> s) # s = t \<lhd> s"
-apply (case_tac "t = Var v")
-apply (erule_tac [2] rev_mp)
-apply (rule_tac [2] P = 
+lemma Var_not_occs: "~ (Var(v) \<prec> t) \<Longrightarrow> t \<lhd> (v,t \<lhd> s) # s = t \<lhd> s"
+  apply (case_tac "t = Var v")
+   prefer 2
+   apply (erule rev_mp)+
+   apply (rule_tac P =
          "%x. x \<noteq> Var v --> ~(Var v \<prec> x) --> x \<lhd> (v,t\<lhd>s) #s = x\<lhd>s" 
        in uterm.induct)
-apply auto 
-done
+     apply auto
+  done
 
 lemma agreement: "(t\<lhd>r = t\<lhd>s) = (\<forall>v \<in> vars_of t. Var v \<lhd> r = Var v \<lhd> s)"
-by (induct_tac "t", auto)
+  by (induct t) auto
 
-lemma repl_invariance: "~ v: vars_of(t) ==> t \<lhd> (v,u)#s = t \<lhd> s"
-by (simp add: agreement)
+lemma repl_invariance: "~ v: vars_of t ==> t \<lhd> (v,u)#s = t \<lhd> s"
+  by (simp add: agreement)
 
-lemma Var_in_subst [rule_format]:
-     "v \<in> vars_of(t) --> w \<in> vars_of(t \<lhd> (v,Var(w))#s)"
-by (induct_tac "t", auto)
+lemma Var_in_subst:
+    "v \<in> vars_of(t) --> w \<in> vars_of(t \<lhd> (v,Var(w))#s)"
+  by (induct t) auto
 
 
 subsection{*Equality between Substitutions*}
 
 lemma subst_eq_iff: "r \<doteq> s = (\<forall>t. t \<lhd> r = t \<lhd> s)"
-by (simp add: subst_eq_def)
+  by (simp add: subst_eq_def)
 
 lemma subst_refl [iff]: "r \<doteq> r"
-by (simp add: subst_eq_iff)
+  by (simp add: subst_eq_iff)
 
 lemma subst_sym: "r \<doteq> s ==> s \<doteq> r"
-by (simp add: subst_eq_iff)
+  by (simp add: subst_eq_iff)
 
 lemma subst_trans: "[| q \<doteq> r; r \<doteq> s |] ==> q \<doteq> s"
-by (simp add: subst_eq_iff)
+  by (simp add: subst_eq_iff)
 
 lemma subst_subst2:
     "[| r \<doteq> s; P (t \<lhd> r) (u \<lhd> r) |] ==> P (t \<lhd> s) (u \<lhd> s)"
-by (simp add: subst_eq_def)
+  by (simp add: subst_eq_def)
 
-lemmas ssubst_subst2 = subst_sym [THEN subst_subst2]
+lemma ssubst_subst2:
+    "[| s \<doteq> r; P (t \<lhd> r) (u \<lhd> r) |] ==> P (t \<lhd> s) (u \<lhd> s)"
+  by (simp add: subst_eq_def)
 
 
 subsection{*Composition of Substitutions*}
@@ -106,92 +101,95 @@ lemma [simp]:
      "((a,b)#al) \<lozenge> bl = (a,b \<lhd> bl) # (al \<lozenge> bl)"
      "sdom([]) = {}"
      "sdom((a,b)#al) = (if Var(a)=b then (sdom al) - {a} else sdom al Un {a})"
-by (simp_all add: comp_def sdom_def) 
+  by (simp_all add: comp_def sdom_def) 
 
 lemma comp_Nil [simp]: "s \<lozenge> [] = s"
-by (induct "s", auto)
+  by (induct s) auto
 
 lemma subst_comp_Nil: "s \<doteq> s \<lozenge> []"
-by simp
+  by simp
 
 lemma subst_comp [simp]: "(t \<lhd> r \<lozenge> s) = (t \<lhd> r \<lhd> s)"
-apply (induct_tac "t")
-apply (simp_all (no_asm_simp))
-apply (induct "r", auto)
-done
+  apply (induct t)
+  apply simp_all
+  apply (induct r)
+   apply auto
+  done
 
 lemma comp_assoc: "(q \<lozenge> r) \<lozenge> s \<doteq> q \<lozenge> (r \<lozenge> s)"
-by (simp add: subst_eq_iff)
+  by (simp add: subst_eq_iff)
 
 lemma subst_cong:
-     "[| theta \<doteq> theta1; sigma \<doteq> sigma1|] 
-      ==> (theta \<lozenge> sigma) \<doteq> (theta1 \<lozenge> sigma1)"
-by (simp add: subst_eq_def)
+  "[| theta \<doteq> theta1; sigma \<doteq> sigma1|] 
+    ==> (theta \<lozenge> sigma) \<doteq> (theta1 \<lozenge> sigma1)"
+  by (simp add: subst_eq_def)
 
 
 lemma Cons_trivial: "(w, Var(w) \<lhd> s) # s \<doteq> s"
-apply (simp add: subst_eq_iff)
-apply (rule allI)
-apply (induct_tac "t", simp_all)
-done
+  apply (simp add: subst_eq_iff)
+  apply (rule allI)
+  apply (induct_tac t)
+    apply simp_all
+  done
 
 
 lemma comp_subst_subst: "q \<lozenge> r \<doteq> s ==>  t \<lhd> q \<lhd> r = t \<lhd> s"
-by (simp add: subst_eq_iff)
+  by (simp add: subst_eq_iff)
 
 
 subsection{*Domain and range of Substitutions*}
 
 lemma sdom_iff: "(v \<in> sdom(s)) = (Var(v) \<lhd> s ~= Var(v))"
-apply (induct "s")
-apply (case_tac [2] a, auto)  
-done
+  apply (induct s)
+   apply (case_tac [2] a)
+   apply auto
+  done
 
 
 lemma srange_iff: 
-   "v \<in> srange(s) = (\<exists>w. w \<in> sdom(s) & v \<in> vars_of(Var(w) \<lhd> s))"
-by (auto simp add: srange_def)
+    "v \<in> srange(s) = (\<exists>w. w \<in> sdom(s) & v \<in> vars_of(Var(w) \<lhd> s))"
+  by (auto simp add: srange_def)
 
 lemma empty_iff_all_not: "(A = {}) = (ALL a.~ a:A)"
-by (unfold empty_def, blast)
+  unfolding empty_def by blast
 
 lemma invariance: "(t \<lhd> s = t) = (sdom(s) Int vars_of(t) = {})"
-apply (induct_tac "t")
-apply (auto simp add: empty_iff_all_not sdom_iff)
-done
+  apply (induct t)
+    apply (auto simp add: empty_iff_all_not sdom_iff)
+  done
 
-lemma Var_in_srange [rule_format]:
-     "v \<in> sdom(s) -->  v \<in> vars_of(t \<lhd> s) --> v \<in> srange(s)"
-apply (induct_tac "t")
-apply (case_tac "a \<in> sdom s")
-apply (auto simp add: sdom_iff srange_iff)
-done
+lemma Var_in_srange:
+    "v \<in> sdom(s) \<Longrightarrow>  v \<in> vars_of(t \<lhd> s) \<Longrightarrow> v \<in> srange(s)"
+  apply (induct t)
+    apply (case_tac "a \<in> sdom s")
+  apply (auto simp add: sdom_iff srange_iff)
+  done
 
 lemma Var_elim: "[| v \<in> sdom(s); v \<notin> srange(s) |] ==>  v \<notin> vars_of(t \<lhd> s)"
-by (blast intro: Var_in_srange)
+  by (blast intro: Var_in_srange)
 
-lemma Var_intro [rule_format]:
-     "v \<in> vars_of(t \<lhd> s) --> v \<in> srange(s) | v \<in> vars_of(t)"
-apply (induct_tac "t")
-apply (auto simp add: sdom_iff srange_iff)
-apply (rule_tac x=a in exI, auto) 
-done
+lemma Var_intro:
+    "v \<in> vars_of(t \<lhd> s) \<Longrightarrow> v \<in> srange(s) | v \<in> vars_of(t)"
+  apply (induct t)
+    apply (auto simp add: sdom_iff srange_iff)
+  apply (rule_tac x=a in exI)
+  apply auto 
+  done
 
 lemma srangeD: "v \<in> srange(s) ==> \<exists>w. w \<in> sdom(s) & v \<in> vars_of(Var(w) \<lhd> s)"
-by (simp add: srange_iff)
+  by (simp add: srange_iff)
 
 lemma dom_range_disjoint:
-     "sdom(s) Int srange(s) = {} = (\<forall>t. sdom(s) Int vars_of(t \<lhd> s) = {})"
-apply (simp add: empty_iff_all_not)
-apply (force intro: Var_in_srange dest: srangeD)
-done
+    "sdom(s) Int srange(s) = {} = (\<forall>t. sdom(s) Int vars_of(t \<lhd> s) = {})"
+  apply (simp add: empty_iff_all_not)
+  apply (force intro: Var_in_srange dest: srangeD)
+  done
 
 lemma subst_not_empty: "~ u \<lhd> s = u ==> (\<exists>x. x \<in> sdom(s))"
-by (auto simp add: empty_iff_all_not invariance)
+  by (auto simp add: empty_iff_all_not invariance)
 
 
 lemma id_subst_lemma [simp]: "(M \<lhd> [(x, Var x)]) = M"
-by (induct_tac "M", auto)
-
+  by (induct M) auto
 
 end
