src/HOL/Subst/Unifier.thy
@@ -8,24 +8,23 @@ header{*Definition of Most General Unifier*}
 
 theory Unifier
 imports Subst
-
 begin
 
-consts
+definition
+  Unifier   :: "[('a * 'a uterm)list, 'a uterm, 'a uterm] => bool" where
+  "Unifier s t u \<longleftrightarrow> t <| s = u <| s"
 
-  Unifier   :: "[('a * 'a uterm)list, 'a uterm, 'a uterm] => bool"
-  ">>"      :: "[('a * 'a uterm)list, ('a * 'a uterm)list] => bool" (infixr 52)
-  MGUnifier :: "[('a * 'a uterm)list, 'a uterm, 'a uterm] => bool"
-  Idem      :: "('a * 'a uterm)list => bool"
+definition
+  MoreGeneral :: "[('a * 'a uterm)list, ('a * 'a uterm)list] => bool" (infixr ">>" 52) where
+  "r >> s \<longleftrightarrow> (\<exists>q. s =$= r <> q)"
 
-defs
+definition
+  MGUnifier :: "[('a * 'a uterm)list, 'a uterm, 'a uterm] => bool" where
+  "MGUnifier s t u \<longleftrightarrow> Unifier s t u & (\<forall>r. Unifier r t u --> s >> r)"
 
-  Unifier_def:      "Unifier s t u == t <| s = u <| s"
-  MoreGeneral_def:  "r >> s == ? q. s =$= r <> q"
-  MGUnifier_def:    "MGUnifier s t u == Unifier s t u & 
-                                        (!r. Unifier r t u --> s >> r)"
-  Idem_def:         "Idem(s) == (s <> s) =$= s"
-
+definition
+  Idem :: "('a * 'a uterm)list => bool" where
+  "Idem s \<longleftrightarrow> (s <> s) =$= s"
 
 
 lemmas unify_defs = Unifier_def MoreGeneral_def MGUnifier_def
@@ -34,62 +33,59 @@ lemmas unify_defs = Unifier_def MoreGeneral_def MGUnifier_def
 subsection{*Unifiers*}
 
 lemma Unifier_Comb [iff]: "Unifier s (Comb t u) (Comb v w) = (Unifier s t v & Unifier s u w)"
-by (simp add: Unifier_def)
+  by (simp add: Unifier_def)
 
 
 lemma Cons_Unifier: "[| v ~: vars_of t; v ~: vars_of u; Unifier s t u |] ==> Unifier ((v,r)#s) t u"
-by (simp add: Unifier_def repl_invariance)
+  by (simp add: Unifier_def repl_invariance)
 
 
 subsection{* Most General Unifiers*}
 
 lemma mgu_sym: "MGUnifier s t u = MGUnifier s u t"
-by (simp add: unify_defs eq_commute)
+  by (simp add: unify_defs eq_commute)
 
 
 lemma MoreGen_Nil [iff]: "[] >> s"
-by (auto simp add: MoreGeneral_def)
+  by (auto simp add: MoreGeneral_def)
 
 lemma MGU_iff: "MGUnifier s t u = (ALL r. Unifier r t u = s >> r)"
-apply (unfold unify_defs)
-apply (auto intro: ssubst_subst2 subst_comp_Nil)
-done
+  apply (unfold unify_defs)
+  apply (auto intro: ssubst_subst2 subst_comp_Nil)
+  done
 
-lemma MGUnifier_Var: "~ Var v <: t ==> MGUnifier [(v,t)] (Var v) t"
-apply (simp (no_asm) add: MGU_iff Unifier_def MoreGeneral_def del: subst_Var)
-apply safe
-apply (rule exI)
-apply (erule subst, rule Cons_trivial [THEN subst_sym])
-apply (erule ssubst_subst2)
-apply (simp (no_asm_simp) add: Var_not_occs)
-done
-
-declare MGUnifier_Var [intro!]
+lemma MGUnifier_Var [intro!]: "~ Var v <: t ==> MGUnifier [(v,t)] (Var v) t"
+  apply (simp (no_asm) add: MGU_iff Unifier_def MoreGeneral_def del: subst_Var)
+  apply safe
+   apply (rule exI)
+   apply (erule subst, rule Cons_trivial [THEN subst_sym])
+  apply (erule ssubst_subst2)
+  apply (simp (no_asm_simp) add: Var_not_occs)
+  done
 
 
 subsection{*Idempotence*}
 
 lemma Idem_Nil [iff]: "Idem([])"
-by (simp add: Idem_def)
+  by (simp add: Idem_def)
 
 lemma Idem_iff: "Idem(s) = (sdom(s) Int srange(s) = {})"
-by (simp add: Idem_def subst_eq_iff invariance dom_range_disjoint)
+  by (simp add: Idem_def subst_eq_iff invariance dom_range_disjoint)
 
 lemma Var_Idem [intro!]: "~ (Var(v) <: t) ==> Idem([(v,t)])"
-by (simp add: vars_iff_occseq Idem_iff srange_iff empty_iff_all_not)
+  by (simp add: vars_iff_occseq Idem_iff srange_iff empty_iff_all_not)
 
 lemma Unifier_Idem_subst: 
   "[| Idem(r); Unifier s (t<|r) (u<|r) |]  
-   ==> Unifier (r <> s) (t <| r) (u <| r)"
-by (simp add: Idem_def Unifier_def comp_subst_subst)
+    ==> Unifier (r <> s) (t <| r) (u <| r)"
+  by (simp add: Idem_def Unifier_def comp_subst_subst)
 
 lemma Idem_comp:
-     "[| Idem(r);  Unifier s (t <| r) (u <| r);  
-         !!q. Unifier q (t <| r) (u <| r) ==> s <> q =$= q  
-      |] ==> Idem(r <> s)"
-apply (frule Unifier_Idem_subst, blast) 
-apply (force simp add: Idem_def subst_eq_iff)
-done
-
+  "[| Idem(r);  Unifier s (t <| r) (u <| r);  
+      !!q. Unifier q (t <| r) (u <| r) ==> s <> q =$= q  
+    |] ==> Idem(r <> s)"
+  apply (frule Unifier_Idem_subst, blast) 
+  apply (force simp add: Idem_def subst_eq_iff)
+  done
 
 end
